# Collision Formulation

$$ f_0^{eq}=w_0\rho [1-\frac{3}{2c^2}(V_x^2+V_y^2)] $$
$$ f_1^{eq}=w_1\rho [1+\frac{3}{c^2}V_x+\frac{9}{2c^2}V_x^2-\frac{3}{2c^2}(V_x^2+V_y^2)] $$
$$ f_2^{eq}=w_2\rho [1+\frac{3}{c^2}V_y+\frac{9}{2c^2}V_y^2-\frac{3}{2c^2}(V_x^2+V_y^2)] $$
$$ f_3^{eq}=w_3\rho [1-\frac{3}{c^2}V_x+\frac{9}{2c^2}V_x^2-\frac{3}{2c^2}(V_x^2+V_y^2)] $$
$$ f_4^{eq}=w_4\rho [1-\frac{3}{c^2}V_y+\frac{9}{2c^2}V_y^2-\frac{3}{2c^2}(V_x^2+V_y^2)] $$
$$ f_5^{eq}=w_5\rho [1+\frac{3}{c^2}(V_x+V_y)+\frac{9}{2c^2}(V_x+V_y)^2-\frac{3}{2c^2}(V_x^2+V_y^2)] $$
$$ f_6^{eq}=w_6\rho [1+\frac{3}{c^2}(-V_x+V_y)+\frac{9}{2c^2}(-V_x+V_y)^2-\frac{3}{2c^2}(V_x^2+V_y^2)] $$
$$ f_7^{eq}=w_7\rho [1+\frac{3}{c^2}(-V_x-V_y)+\frac{9}{2c^2}(-V_x-V_y)^2-\frac{3}{2c^2}(V_x^2+V_y^2)] $$
$$ f_8^{eq}=w_8\rho [1+\frac{3}{c^2}(V_x-V_y)+\frac{9}{2c^2}(V_x-V_y)^2-\frac{3}{2c^2}(V_x^2+V_y^2)] $$

